Clap/Lang/Wheels.lean
@@ -5,4 +5,8 @@ namespace Clap
 attribute [simp]
   sub_eq_zero
 
+attribute [grind =]
+  Option.isSome_eq_false_iff
+  Option.isNone_iff_eq_none
+
 end Clap
